

Unitary Time Changes of Stationary Processes Yield Oscillatory Processes

BY STEPHEN CROWLEY

September 16, 2025

Table of contents

1 Oscillatory Processes	1
2 Unitarily Time-Changed Stationary Processes	5
2.1 Unitary Time-Change Operator $U_\theta f$	5
2.2 Transformation of Stationary \rightarrow Oscillatory Processes via U_θ	7
2.2.1 Time-Varying Filter Representations	9
2.3 Covariance operator conjugation	9
Bibliography	10

1 Oscillatory Processes

Remark 1. Unless otherwise stated.

1. All parametric families $\{f_t(\omega)\}$ are jointly measurable with respect to $\mathcal{B}(\mathbb{R}) \otimes \mathcal{B}(\mathbb{R})$.
2. Dirac delta identities such as $\int e^{i(\mu-\lambda)u} du = 2\pi \delta(\mu - \lambda)$ are distributional.
3. Integrals of the form $\int f(\omega) d\nu(\omega)$ denote Lebesgue-Stieltjes integration with respect to measure ν , while $\int g(u) du$ denotes Lebesgue integration with respect to Lebesgue measure.
4. Integrals with respect to orthogonal random measures Φ , written $\int h(\omega) d\Phi(\omega)$, are Lebesgue-Stieltjes integrals in $L^2(\Omega)$ with variance $\mathbb{E}[|\int h d\Phi|^2] = \int |h|^2 d\mu$.
5. Limit interchange is justified by dominated convergence under uniform L^2 bounds.

Throughout, $(\Omega, \mathcal{F}, \mathbb{P})$ is a fixed probability space and μ is a finite Borel measure on \mathbb{R} .

Definition 2. [*Oscillatory process*] [2] Let F be a finite nonnegative Borel measure on \mathbb{R} . Let the gain function be

$$A_t(\lambda) \in L^2(F) \quad \forall t, \lambda \in \mathbb{R} \quad (1)$$

so that the corresponding oscillatory function is given by

$$\varphi_t(\lambda) = A_t(\lambda) e^{i\lambda t} \in L^2(F) \text{ since } |e^{i\lambda t}| = 1 \forall t, \lambda \in \mathbb{R} \quad (2)$$

then an oscillatory process is a (non-stationary) Gaussian process which can be represented as

$$\begin{aligned} Z(t) &= \int_{-\infty}^{\infty} \varphi_t(\lambda) d\Phi(\lambda) \\ &= \int_{-\infty}^{\infty} A_t(\lambda) e^{i\lambda t} d\Phi(\lambda) \end{aligned} \quad (3)$$

where Φ is a complex orthogonal random measure with spectral measure F which satisfies the relation

$$d\mathbb{E}[\Phi(\lambda)\overline{\Phi(\mu)}] = \delta(\lambda - \mu) dF(\lambda) \quad (4)$$

and has the corresponding covariance kernel

$$\begin{aligned} R_Z(t, s) &= \mathbb{E}[Z(t)\overline{Z(s)}] \\ &= \int_{\mathbb{R}} A_t(\lambda)\overline{A_s(\lambda)} e^{i\lambda(t-s)} dF(\lambda) \\ &= \int_{\mathbb{R}} \varphi_t(\lambda)\overline{\varphi_s(\lambda)} dF(\lambda) \end{aligned} \quad (5)$$

Theorem 3. [*Quadratic Integrability Condition*] Let $(\Omega, \mathcal{A}, \mu)$ be a σ -finite measure space and Φ a complex-valued orthogonal random measure with second moment measure μ . Let $A: \mathbb{R} \times \Omega \rightarrow \mathbb{C}$ be measurable in each variable and define $\varphi_t(\omega) = A(t, \omega) e^{i\omega t}$. Then for each fixed $t \in \mathbb{R}$, the stochastic integral

$$X_t = \int_{\Omega} \varphi_t(\omega) d\Phi(\omega) \quad (6)$$

exists if and only if φ_t is square-integrable with respect to μ :

$$\int_{\Omega} |\varphi_t(\omega)|^2 d\mu(\omega) < \infty. \quad (7)$$

Equivalently, since $|e^{i\omega t}| = 1$, this condition reduces to

$$\int_{\Omega} |A(t, \omega)|^2 d\mu(\omega) < \infty. \quad (8)$$

Proof. For each fixed t , we have the algebraic identity

$$|\varphi_t(\omega)|^2 = |A(t, \omega) e^{i\omega t}|^2 = |A(t, \omega)|^2 \cdot |e^{i\omega t}|^2 = |A(t, \omega)|^2. \quad (9)$$

Therefore

$$\int_{\Omega} |\varphi_t(\omega)|^2 d\mu(\omega) = \int_{\Omega} |A(t, \omega)|^2 d\mu(\omega). \quad (10)$$

The stochastic integral X_t is defined via the Itô isometry:

$$\mathbb{E} \left[\left| \int_{\Omega} \varphi_t(\omega) d\Phi(\omega) \right|^2 \right] = \int_{\Omega} |\varphi_t(\omega)|^2 d\mu(\omega). \quad (11)$$

Hence the integral exists in $L^2(\Omega)$ precisely when the right-hand side is finite. The condition on $A(t, \cdot)$ follows immediately. \square

Theorem 4. [Real-valuedness criterion for oscillatory processes] *Let Z be an oscillatory process with oscillatory function*

$$\varphi_t(\lambda) = A_t(\lambda) e^{i\lambda t} \quad (12)$$

and spectral measure F . Then Z is real-valued if and only if

$$A_t(-\lambda) = \overline{A_t(\lambda)} \quad (13)$$

for F -almost every $\lambda \in \mathbb{R}$, equivalently

$$\varphi_t(-\lambda) = \overline{\varphi_t(\lambda)} \quad (14)$$

for F -almost every $\lambda \in \mathbb{R}$.

Proof. 1. Assume Z is real-valued. Then for all $t \in \mathbb{R}$,

$$Z(t) = \overline{Z(t)} \quad (15)$$

2. From the oscillatory representation (3),

$$Z(t) = \int_{\mathbb{R}} A_t(\lambda) e^{i\lambda t} d\Phi(\lambda) \quad (16)$$

3. Taking the complex conjugate of both sides of (16),

$$\overline{Z(t)} = \overline{\int_{\mathbb{R}} A_t(\lambda) e^{i\lambda t} d\Phi(\lambda)} = \int_{\mathbb{R}} \overline{A_t(\lambda)} e^{-i\lambda t} d\overline{\Phi(\lambda)} \quad (17)$$

4. For a real-valued process, the orthogonal random measure must satisfy the symmetry property

$$d\overline{\Phi(\lambda)} = d\Phi(-\lambda) \quad (18)$$

5. Substituting (18) into (17),

$$\overline{Z(t)} = \int_{\mathbb{R}} \overline{A_t(\lambda)} e^{-i\lambda t} d\Phi(-\lambda) \quad (19)$$

6. Apply the change of variables $\mu = -\lambda$, so $d\Phi(-\lambda) = d\Phi(\mu)$ and $e^{-i\lambda t} = e^{i\mu t}$:

$$\overline{Z(t)} = \int_{\mathbb{R}} \overline{A_t(-\mu)} e^{i\mu t} d\Phi(\mu) \quad (20)$$

7. By (15), the right sides of (16) and (20) must be equal:

$$\int_{\mathbb{R}} A_t(\mu) e^{i\mu t} d\Phi(\mu) = \int_{\mathbb{R}} \overline{A_t(-\mu)} e^{i\mu t} d\Phi(\mu) \quad (21)$$

8. Since the stochastic integral representation is unique in $L^2(F)$, the integrands must be equal F -almost everywhere:

$$A_t(\lambda) = \overline{A_t(-\lambda)} \quad \text{for } F\text{-a.e. } \lambda \quad (22)$$

9. This is equivalent to (13). From (12),

$$\varphi_t(-\lambda) = A_t(-\lambda) e^{-i\lambda t} \quad (23)$$

10. Using (13),

$$\begin{aligned} \varphi_t(-\lambda) &= \overline{A_t(\lambda)} e^{-i\lambda t} \\ &= \overline{A_t(\lambda)} e^{i\lambda t} \\ &= \varphi_t(\lambda) \end{aligned} \quad (24)$$

establishing (14).

11. Conversely, assume (13) holds. Reversing the steps from (20) to (15) shows that $\overline{Z(t)} = Z(t)$ for all t , so Z is real-valued. \square

Theorem 5. [Filter representation] Let X be a zero-mean stationary process

$$X(u) = \int e^{i\lambda u} d\Phi(\lambda) \quad (25)$$

and spectral measure F , and let Z be an oscillatory process with oscillatory function $\varphi_t(\lambda)$ and the same orthogonal random measure Φ . Then

$$Z(t) = \int_{-\infty}^{\infty} h(t, u) X(u) du \quad (26)$$

where

$$h(t, u) = \frac{1}{2\pi} \int_{-\infty}^{\infty} \varphi_t(\lambda) e^{-i\lambda u} d\lambda \quad (27)$$

where $h(t, u)$ is the forward impulse response of Definition ?.

Proof. 1. Substitute the definitions of $h(t, u)$ and $X(u)$:

$$\int_{-\infty}^{\infty} h(t, u) X(u) du = \int_{-\infty}^{\infty} \left[\frac{1}{2\pi} \int_{-\infty}^{\infty} \varphi_t(\lambda) e^{-i\lambda u} d\lambda \right] \left[\int_{-\infty}^{\infty} e^{i\mu u} d\Phi(\mu) \right] du \quad (28)$$

2. Apply Fubini's theorem:

$$= \frac{1}{2\pi} \int_{-\infty}^{\infty} \int_{-\infty}^{\infty} \varphi_t(\lambda) \left[\int_{-\infty}^{\infty} e^{i(\mu-\lambda)u} du \right] d\lambda d\Phi(\mu) \quad (29)$$

3. The inner integral over u is the Fourier representation of the Dirac delta:

$$\int_{-\infty}^{\infty} e^{i(\mu-\lambda)u} du = 2\pi \delta(\mu - \lambda) \quad (30)$$

4. Substitute:

$$= \frac{1}{2\pi} \int_{-\infty}^{\infty} \int_{-\infty}^{\infty} \varphi_t(\lambda) \cdot 2\pi \delta(\mu - \lambda) d\lambda d\Phi(\mu) \quad (31)$$

5. Simplify:

$$= \int_{-\infty}^{\infty} \int_{-\infty}^{\infty} \varphi_t(\lambda) \delta(\mu - \lambda) d\lambda d\Phi(\mu) \quad (32)$$

6. Apply the sifting property of the delta function:

$$= \int_{-\infty}^{\infty} \varphi_t(\mu) d\Phi(\mu) = Z(t) \quad (33) \quad \square$$

2 Unitarily Time-Changed Stationary Processes

2.1 Unitary Time-Change Operator $U_\theta f$

Theorem 6. *[Unitary time-change operator U_θ and its inverse U_θ^{-1}] Let the time-change function $\theta: \mathbb{R} \rightarrow \mathbb{R}$ be absolutely continuous, strictly increasing, and bijective, with*

$$\dot{\theta}(t) > 0 \quad (34)$$

almost everywhere and $\dot{\theta}(t) = 0$ only on sets of Lebesgue measure zero. For f measurable, define

$$(U_\theta f)(t) = \sqrt{\dot{\theta}(t)} f(\theta(t)) \quad (35)$$

Its inverse is given by

$$(U_\theta^{-1} g)(s) = \frac{g(\theta^{-1}(s))}{\sqrt{\dot{\theta}(\theta^{-1}(s))}} \quad (36)$$

For every compact set $K \subseteq \mathbb{R}$ and $f \in L^2_{\text{loc}}(\mathbb{R})$,

$$\int_K |(U_\theta f)(t)|^2 dt = \int_{\theta(K)} |f(s)|^2 ds \quad (37)$$

Moreover, U_θ^{-1} is the inverse of U_θ on $L^2_{\text{loc}}(\mathbb{R})$.

Proof. 1. Let $f \in L^2_{\text{loc}}(\mathbb{R})$ and let $K \subset \mathbb{R}$ be compact. From the definition (35),

$$\int_K |(U_\theta f)(t)|^2 dt = \int_K \left| \sqrt{\dot{\theta}(t)} f(\theta(t)) \right|^2 dt \quad (38)$$

2. Expanding the square,

$$\int_K \left| \sqrt{\dot{\theta}(t)} f(\theta(t)) \right|^2 dt = \int_K \dot{\theta}(t) |f(\theta(t))|^2 dt \quad (39)$$

3. Since θ is absolutely continuous and strictly increasing, $\theta' = \dot{\theta}$ exists almost everywhere and $\dot{\theta}(t) > 0$ a.e.

4. Apply the change of variables $s = \theta(t)$. Then

$$ds = \dot{\theta}(t) dt \quad (40)$$

5. The inverse function $t = \theta^{-1}(s)$ exists since θ is strictly increasing and bijective.

6. As t ranges over K , the variable $s = \theta(t)$ ranges over $\theta(K)$.

7. Since θ is continuous and K is compact, $\theta(K)$ is compact.

8. Substituting (40) into (39),

$$\int_K \dot{\theta}(t) |f(\theta(t))|^2 dt = \int_{\theta(K)} |f(s)|^2 ds \quad (41)$$

9. This establishes the local isometry (37).

10. To verify U_θ^{-1} is the inverse, compute:

$$(U_\theta^{-1} U_\theta f)(s) = U_\theta^{-1} (U_\theta f)(s) \quad (42)$$

11. By definition (36),

$$U_\theta^{-1} (U_\theta f)(s) = \frac{(U_\theta f)(\theta^{-1}(s))}{\sqrt{\dot{\theta}(\theta^{-1}(s))}} \quad (43)$$

12. By definition (35),

$$(U_\theta f)(\theta^{-1}(s)) = \sqrt{\dot{\theta}(\theta^{-1}(s))} f(\theta(\theta^{-1}(s))) \quad (44)$$

13. Since $\theta \circ \theta^{-1} = \text{id}$,

$$f(\theta(\theta^{-1}(s))) = f(s) \quad (45)$$

14. Substituting (44) and (45) into (43),

$$\frac{\sqrt{\dot{\theta}(\theta^{-1}(s))} f(s)}{\sqrt{\dot{\theta}(\theta^{-1}(s))}} = f(s) \quad (46)$$

15. Therefore

$$U_\theta^{-1} U_\theta = \text{id} \quad (47)$$

16. Similarly, compute:

$$(U_\theta U_\theta^{-1} g)(t) = \sqrt{\dot{\theta}(t)} (U_\theta^{-1} g)(\theta(t)) \quad (48)$$

17. By definition (36),

$$(U_\theta^{-1} g)(\theta(t)) = \frac{g(\theta^{-1}(\theta(t)))}{\sqrt{\dot{\theta}(\theta^{-1}(\theta(t)))}} \quad (49)$$

18. Since $\theta^{-1} \circ \theta = \text{id}$,

$$g(\theta^{-1}(\theta(t))) = g(t), \quad \theta^{-1}(\theta(t)) = t \quad (50)$$

19. Substituting (50) into (49),

$$\frac{g(t)}{\sqrt{\dot{\theta}(t)}} \quad (51)$$

20. Therefore from (48),

$$(U_\theta U_\theta^{-1} g)(t) = \sqrt{\dot{\theta}(t)} \cdot \frac{g(t)}{\sqrt{\dot{\theta}(t)}} = g(t) \quad (52)$$

21. Thus

$$U_\theta U_\theta^{-1} = \text{id} \quad (53)$$

22. Combining (47) and (53), U_θ^{-1} is the two-sided inverse of U_θ on $L^2_{\text{loc}}(\mathbb{R})$. \square

2.2 Transformation of Stationary \rightarrow Oscillatory Processes via U_θ

Theorem 7. *[Unitary time changes of stationary processes produce oscillatory process] Let X be zero-mean stationary as in Definition ?. For scaling function θ as in Theorem 6, define*

$$\begin{aligned} Z(t) &= (U_\theta X)(t) \\ &= \sqrt{\dot{\theta}(t)} X(\theta(t)) \end{aligned} \quad (54)$$

Then Z is a realization of an oscillatory process with oscillatory function

$$\varphi_t(\lambda) = \sqrt{\dot{\theta}(t)} e^{i\lambda\theta(t)} \quad (55)$$

gain function

$$A_t(\lambda) = \sqrt{\dot{\theta}(t)} e^{i\lambda(\theta(t)-t)} \quad (56)$$

and covariance kernel

$$\begin{aligned} R_Z(t, s) &= \mathbb{E}[Z(t)\overline{Z(s)}] \\ &= \mathbb{E}\left[\sqrt{\dot{\theta}(t)} X(\theta(t)) \sqrt{\dot{\theta}(s)} \overline{X(\theta(s))}\right] \\ &= \sqrt{\dot{\theta}(t)\dot{\theta}(s)} \mathbb{E}[X(\theta(t))\overline{X(\theta(s))}] \\ &= \sqrt{\dot{\theta}(t)\dot{\theta}(s)} R_X(\theta(t) - \theta(s)) \\ &= \sqrt{\dot{\theta}(t)\dot{\theta}(s)} \int_{\mathbb{R}} e^{i\lambda(\theta(t)-\theta(s))} dF(\lambda) \end{aligned} \quad (57)$$

Proof. 1. From the Cramér representation (?),

$$X(u) = \int_{\mathbb{R}} e^{i\lambda u} d\Phi(\lambda) \quad (58)$$

2. Substituting $u = \theta(t)$ into (58),

$$X(\theta(t)) = \int_{\mathbb{R}} e^{i\lambda\theta(t)} d\Phi(\lambda) \quad (59)$$

3. From the definition (54),

$$Z(t) = \sqrt{\dot{\theta}(t)} X(\theta(t)) = \sqrt{\dot{\theta}(t)} \int_{\mathbb{R}} e^{i\lambda\theta(t)} d\Phi(\lambda) \quad (60)$$

4. By linearity of the stochastic integral,

$$Z(t) = \int_{\mathbb{R}} \sqrt{\dot{\theta}(t)} e^{i\lambda\theta(t)} d\Phi(\lambda) \quad (61)$$

5. Define

$$\varphi_t(\lambda) := \sqrt{\dot{\theta}(t)} e^{i\lambda\theta(t)} \quad (62)$$

6. Then (61) becomes

$$Z(t) = \int_{\mathbb{R}} \varphi_t(\lambda) d\Phi(\lambda) \quad (63)$$

which is the oscillatory representation (3).

7. To express this in terms of the standard oscillatory function form, define the gain function

$$A_t(\lambda) = \sqrt{\dot{\theta}(t)} e^{i\lambda(\theta(t)-t)} \quad (64)$$

8. Then verify the oscillatory function form (2) factorizes

$$\begin{aligned} \varphi_t(\lambda) &= A_t(\lambda) e^{i\lambda t} \\ &= \sqrt{\dot{\theta}(t)} e^{i\lambda(\theta(t)-t)} e^{i\lambda t} \\ &= \sqrt{\dot{\theta}(t)} e^{i\lambda(\theta(t)-t+t)} \\ &= \sqrt{\dot{\theta}(t)} e^{i\lambda\theta(t)} \end{aligned} \quad (65)$$

9. To compute the covariance, use (5):

$$R_Z(t, s) = \mathbb{E}[Z(t)\overline{Z(s)}] \quad (66)$$

10. Substituting (54),

$$R_Z(t, s) = \mathbb{E} \left[\sqrt{\dot{\theta}(t)} X(\theta(t)) \overline{\sqrt{\dot{\theta}(s)} X(\theta(s))} \right] \quad (67)$$

11. Since $\dot{\theta}$ is deterministic,

$$R_Z(t, s) = \sqrt{\dot{\theta}(t)} \sqrt{\dot{\theta}(s)} \mathbb{E}[X(\theta(t))\overline{X(\theta(s))}] \quad (68)$$

12. By stationarity of X ,

$$\mathbb{E}[X(\theta(t))\overline{X(\theta(s))}] = R_X(\theta(t) - \theta(s)) = \int_{\mathbb{R}} e^{i\lambda(\theta(t)-\theta(s))} dF(\lambda) \quad (69)$$

13. Substituting (69) into (68),

$$R_Z(t, s) = \sqrt{\dot{\theta}(t)\dot{\theta}(s)} \int_{\mathbb{R}} e^{i\lambda(\theta(t)-\theta(s))} dF(\lambda) \quad (70)$$

establishing (57). \square

Corollary 8. *The evolutionary spectrum is*

$$dF_t(\lambda) = \dot{\theta}(t) dF(\lambda) \quad (71)$$

Proof. 1. The evolutionary spectrum is defined by

$$dF_t(\lambda) = |A_t(\lambda)|^2 dF(\lambda) \quad (72)$$

2. From (56),

$$|A_t(\lambda)|^2 = \left| \sqrt{\dot{\theta}(t)} e^{i\lambda(\theta(t)-t)} \right|^2 \quad (73)$$

3. Since $|e^{i\alpha}| = 1$ for all real α ,

$$|e^{i\lambda(\theta(t)-t)}|^2 = 1 \quad (74)$$

4. Therefore

$$|A_t(\lambda)|^2 = \left(\sqrt{\dot{\theta}(t)} \right)^2 \cdot 1 = \dot{\theta}(t) \quad (75)$$

5. Substituting (75) into (72),

$$dF_t(\lambda) = \dot{\theta}(t) dF(\lambda) \quad (76) \quad \square$$

2.2.1 Time-Varying Filter Representations

... not necessary ...

2.3 Covariance operator conjugation

Proposition 9. *Let*

$$(T_K f)(t) := \int_{\mathbb{R}} K(|t-s|) f(s) ds \quad (77)$$

with stationary kernel

$$K(h) = \int_{\mathbb{R}} e^{i\lambda h} dF(\lambda) \quad (78)$$

Define the transformed kernel

$$\begin{aligned} K_\theta(s, t) &= (U_{t \rightarrow \theta(t)} (U_{s \rightarrow \theta(s)} K))(t, s) \\ &= (U_{s \rightarrow \theta(s)} (U_{t \rightarrow \theta(t)} K))(t, s) \\ &= \sqrt{\dot{\theta}(t) \dot{\theta}(s)} K(|\theta(t) - \theta(s)|) \end{aligned} \quad (79)$$

then the corresponding integral covariance operator is conjugated for all $f \in L^2_{\text{loc}}(\mathbb{R})$ by

$$(T_{K_\theta} f)(t) = (U_\theta T_K U_\theta^{-1} f)(t) \quad (80)$$

Proof. 1. From (80), expand the right side:

$$(U_\theta T_K U_\theta^{-1} f)(t) = \sqrt{\dot{\theta}(t)} (T_K U_\theta^{-1} f)(\theta(t)) \quad (81)$$

2. By definition (77),

$$(T_K U_\theta^{-1} f)(\theta(t)) = \int_{\mathbb{R}} K(|\theta(t) - s|) (U_\theta^{-1} f)(s) ds \quad (82)$$

3. By definition (36),

$$(U_\theta^{-1} f)(s) = \frac{f(\theta^{-1}(s))}{\sqrt{\dot{\theta}(\theta^{-1}(s))}} \quad (83)$$

4. Substituting (83) into (82),

$$\int_{\mathbb{R}} K(|\theta(t) - s|) \frac{f(\theta^{-1}(s))}{\sqrt{\dot{\theta}(\theta^{-1}(s))}} ds \quad (84)$$

5. Apply the change of variables $s = \theta(u)$, so $ds = \dot{\theta}(u) du$ and $\theta^{-1}(s) = u$:

$$\int_{\mathbb{R}} K(|\theta(t) - \theta(u)|) \frac{f(u)}{\sqrt{\dot{\theta}(u)}} \dot{\theta}(u) du \quad (85)$$

6. Simplify:

$$\int_{\mathbb{R}} K(|\theta(t) - \theta(u)|) \frac{\dot{\theta}(u)}{\sqrt{\dot{\theta}(u)}} f(u) du = \int_{\mathbb{R}} K(|\theta(t) - \theta(u)|) \sqrt{\dot{\theta}(u)} f(u) du \quad (86)$$

7. Substituting (86) into (81),

$$\sqrt{\dot{\theta}(t)} \int_{\mathbb{R}} K(|\theta(t) - \theta(u)|) \sqrt{\dot{\theta}(u)} f(u) du \quad (87)$$

8. Bring the constant inside the integral:

$$\int_{\mathbb{R}} \sqrt{\dot{\theta}(t)} \sqrt{\dot{\theta}(u)} K(|\theta(t) - \theta(u)|) f(u) du \quad (88)$$

9. Combine the square roots $\sqrt{\dot{\theta}(t)} \sqrt{\dot{\theta}(u)} = \sqrt{\dot{\theta}(t)\dot{\theta}(s)}$ and recognize definition (79),

$$\sqrt{\dot{\theta}(t)\dot{\theta}(s)} K(|\theta(t) - \theta(u)|) = K_\theta(u, t) \quad (89)$$

10. Therefore

$$\begin{aligned} \int_{\mathbb{R}} K_\theta(u, t) f(u) du &= \int_{\mathbb{R}} \sqrt{\dot{\theta}(t)\dot{\theta}(s)} K(|\theta(t) - \theta(u)|) f(u) du \\ &= (T_{K_\theta} f)(t) \end{aligned} \quad (90)$$

establishing (80). □

Bibliography

- [1] Harald Cramér and M.R. Leadbetter. *Stationary and Related Processes: Sample Function Properties and Their Applications*. Wiley Series in Probability and Mathematical Statistics. 1967.
- [2] Maurice B Priestley. Evolutionary spectra and non-stationary processes. *Journal of the Royal Statistical Society: Series B (Methodological)*, 27(2):204–229, 1965.